pulse/ulib/experimental/Steel.C.Frac.fsti
@@ -46,15 +46,15 @@ let frac_pcm_fpu
 = base_fpu pcm_frac x (Some (y, full_perm))
 
 val frac_pcm_write
-  (#a:Type) (#b: Type)
-  (r: ref a (pcm_frac #b)) (x: Ghost.erased (fractional b)) (y: b)
+  (#b: Type)
+  (r: ref (pcm_frac #b)) (x: Ghost.erased (fractional b)) (y: b)
 : Steel unit (r `pts_to` x) (fun _ -> r `pts_to` Some (y, full_perm))
   (requires (fun _ -> Some? x /\ snd (Some?.v x) == full_perm))
   (ensures (fun _ _ _ -> True))
 
 val frac_pcm_read
-  (#a:Type) (#b: Type)
-  (r: ref a (pcm_frac #b)) (x: Ghost.erased (fractional b))
+  (#b: Type)
+  (r: ref (pcm_frac #b)) (x: Ghost.erased (fractional b))
 : Steel b (r `pts_to` x) (fun _ -> r `pts_to` x)
   (requires (fun _ -> Some? x))
   (ensures (fun _ y _ -> Some? x /\ y == fst (Some?.v (Ghost.reveal x))))
@@ -78,9 +78,9 @@ let frac_view
 }
 
 let frac_read_sel
-  (#a: Type u#0) (#b: Type u#0)
+  (#b: Type u#0)
   (#p: perm)
-  (r: ref a (pcm_frac #b))
+  (r: ref (pcm_frac #b))
 : Steel b
   (pts_to_view r (frac_view _ p))
   (fun _ -> pts_to_view r (frac_view _ p))
@@ -92,9 +92,9 @@ let frac_read_sel
 = ref_read_sel r (frac_view _ p)
 
 let frac_write_sel
-  (#a: Type u#0) (#b: Type u#0)
+  (#b: Type u#0)
   (#p: perm)
-  (r: ref a (pcm_frac #b))
+  (r: ref (pcm_frac #b))
   (w: b)
 : Steel unit
   (pts_to_view r (frac_view _ p))
