pulse/ulib/experimental/Steel.C.StructLiteral.fsti
@@ -268,13 +268,12 @@ val extract_field_unextracted'
 val addr_of_struct_field_ref
   (#tag: Type0) (#fields: c_fields) (#excluded: excluded_fields)
   (field: field_of fields)
-  (p: ref 'a (struct_pcm tag fields))
-: Steel (ref 'a (fields.get_field field).pcm)
+  (p: ref (struct_pcm tag fields))
+: Steel (ref (fields.get_field field).pcm)
     (p `pts_to_view` struct_view tag fields excluded)
     (fun q ->
       (p `pts_to_view` struct_view tag fields (insert field excluded)) `star`
       (pts_to_view u#0
-                  #'a
                   #(norm simplify_typedefs (norm unfold_typedefs (fields.get_field field).carrier))
                   #(norm simplify_typedefs (norm unfold_typedefs (fields.get_field field).pcm))
                   q
@@ -295,8 +294,8 @@ val addr_of_struct_field_ref
 val unaddr_of_struct_field_ref'
   (#tag: Type0) (#fields: c_fields) (#excluded: excluded_fields)
   (field: field_of fields)
-  (p: ref 'a (struct_pcm tag fields))
-  (q: ref 'a (fields.get_field field).pcm)
+  (p: ref (struct_pcm tag fields))
+  (q: ref (fields.get_field field).pcm)
 : Steel unit
     ((p `pts_to_view` struct_view tag fields excluded) `star`
      (q `pts_to_view` (fields.get_field field).view))
@@ -322,12 +321,11 @@ val dummy_def : unit
 val unaddr_of_struct_field_ref
   (#tag: Type0) (#fields: c_fields) (#excluded: excluded_fields)
   (field: field_of fields)
-  (p: ref 'a (struct_pcm tag fields))
-  (q: ref 'a (fields.get_field field).pcm)
+  (p: ref (struct_pcm tag fields))
+  (q: ref (fields.get_field field).pcm)
 : Steel unit
     ((p `pts_to_view` struct_view tag fields excluded) `star`
      (pts_to_view u#0
-                  #'a
                   #(norm simplify_typedefs (norm unfold_typedefs (fields.get_field field).carrier))
                   #(norm simplify_typedefs (norm unfold_typedefs (fields.get_field field).pcm))
                   q
@@ -359,13 +357,12 @@ let addr_of_struct_field''
   (field: field_of fields{
     return_view_type == (fields.get_field field).view_type /\
     return_carrier == (fields.get_field field).carrier})
-  (p: ref 'a (struct tag fields) (struct_pcm tag fields))
-: Steel (ref 'a return_view_type #return_carrier (fields.get_field field).pcm)
+  (p: ref (struct tag fields) (struct_pcm tag fields))
+: Steel (ref return_view_type #return_carrier (fields.get_field field).pcm)
     (p `pts_to_view` struct_view tag fields excluded)
     (fun q ->
       (p `pts_to_view` struct_view tag fields (insert field excluded)) `star`
       (pts_to_view u#0
-                  #'a
                   #(norm simplify_typedefs (norm unfold_typedefs (fields.get_field field).view_type))
                   #(norm simplify_typedefs (norm unfold_typedefs (fields.get_field field).view_type))
                   #(norm simplify_typedefs (norm unfold_typedefs (fields.get_field field).carrier))
@@ -384,7 +381,7 @@ let addr_of_struct_field''
         snd (extract_field tag fields excluded field
         (h (p `pts_to_view` struct_view tag fields excluded))) ==
          h' (q `pts_to_view` (fields.get_field field).view))
-= addr_of_struct_field_ref #'a #tag #fields #excluded field p
+= addr_of_struct_field_ref #tag #fields #excluded field p
 
 (** Take the address of a field of a struct.
     The above definitions are set up so that calls to addr_of_struct_field are erased to calls to addr_of_struct_field'' with
@@ -402,8 +399,8 @@ inline_for_extraction noextract
 let addr_of_struct_field
   (#tag: Type0) (#fields: c_fields) (#excluded: excluded_fields)
   (field: field_of fields)
-  (p: ref 'a (struct tag fields) (struct_pcm tag fields))
-: Steel (ref 'a
+  (p: ref (struct tag fields) (struct_pcm tag fields))
+: Steel (ref
           (norm simplify_typedefs (fields.get_field field).view_type)
           #(norm simplify_typedefs (fields.get_field field).carrier)
           (fields.get_field field).pcm)
@@ -411,7 +408,6 @@ let addr_of_struct_field
     (fun q ->
       (p `pts_to_view` struct_view tag fields (insert field excluded)) `star`
       (pts_to_view u#0
-                  #'a
                   #(norm simplify_typedefs (norm unfold_typedefs (fields.get_field field).view_type))
                   #(norm simplify_typedefs (norm unfold_typedefs (fields.get_field field).view_type))
                   #(norm simplify_typedefs (norm unfold_typedefs (fields.get_field field).carrier))
@@ -438,14 +434,13 @@ let addr_of_struct_field
 let unaddr_of_struct_field
   (#tag: Type0) (#fields: c_fields) (#excluded: excluded_fields)
   (field: field_of fields)
-  (p: ref 'a (struct tag fields) (struct_pcm tag fields))
-  (q: ref 'a
+  (p: ref (struct tag fields) (struct_pcm tag fields))
+  (q: ref
     (norm simplify_typedefs (norm unfold_typedefs (fields.get_field field).view_type))
     (fields.get_field field).pcm)
 : Steel unit
     ((p `pts_to_view` struct_view tag fields excluded) `star`
      (pts_to_view u#0
-                  #'a
                   #(norm simplify_typedefs (norm unfold_typedefs (fields.get_field field).view_type))
                   #(norm simplify_typedefs (norm unfold_typedefs (fields.get_field field).view_type))
                   #(norm simplify_typedefs (norm unfold_typedefs (fields.get_field field).carrier))
