pulse/ulib/experimental/Steel.PCMReadOnly.fst
@@ -1,0 +1,34 @@
+module Steel.PCMReadOnly
+include FStar.PCM
+
+let readonly (a:Type u#a) = option a
+let composable #a : symrel (readonly a) =
+  fun (f0 f1:readonly a) ->
+    match f0, f1 with
+    | None, _
+    | _, None -> True
+    | Some x0, Some x1 -> x0==x1
+let compose #a (f0:readonly a) (f1:readonly a{composable f0 f1}) : readonly a =
+  match f0, f1 with
+  | None, f
+  | f, None -> f
+  | Some x0, Some _ -> Some x0
+
+let pcm_readonly #a : pcm (readonly a) = {
+  p = {
+         composable = composable;
+         op = compose;
+         one = None
+      };
+  comm = (fun _ _ -> ());
+  assoc = (fun _ _ _ -> ());
+  assoc_r = (fun _ _ _ -> ());
+  is_unit = (fun _ -> ());
+  refine = (fun _ -> True)
+}
+
+let mk_frame_preserving_upd
+  (#a: Type)
+  (v0: a)
+: Tot (frame_preserving_upd pcm_readonly (Some v0) (Some v0))
+= fun _ -> Some v0
